\renewcommand{\familydefault}{\sfdefault}
\documentclass{scrartcl}
\usepackage{amsmath}
\usepackage[utf8]{inputenc}
\usepackage{natbib}
\usepackage{graphicx}
\usepackage[margin=1.2in]{geometry}
\usepackage{wrapfig}

\begin{document}
\title{SYPT Week 6 - Collision}
\author{Li XinRui}
\date{08 12 2020}
\setlength\parindent{0pt}

\maketitle
\section{Kinematics}
$$\omega=\dot\phi$$
$$\alpha=\ddot\phi$$
Centre of Mass:
$$
    \begin{cases}
      \ddot{y}_{\textsf{c}}=\ddot{y}_{\textsf{p}}+\ddot \phi \, \ell \sin\phi-\dot \phi^2 \ell \cos\phi\\
      \ddot{x}_{\textsf{c}}=\ddot{x}_{\textsf{p}}+\ddot \phi \, \ell \cos \phi+ \dot \phi^2 \ell \sin\phi
    \end{cases}    
$$


\section{Dynamics}
\subsection{Spring-Mass-Damper}
$$N-mg=m\ddot{y}_{\textsf{c}}$$
$$N-mg=m(\boxed{\ddot{y}_{\textsf{p}}}+\boxed{\ddot \phi} \ell \sin\phi-\dot \phi^2 \ell \cos\phi)$$
Finding $\ddot{y}_{\textsf{p}}$:
$$
\boxed{
\begin{aligned}
m\ddot{y}_{\textsf{p}}=-mg-kx^\frac{3}{2}-c\dot{y}_{\textsf{p}}\\
\boxed{\ddot{y}_{\textsf{p}}}=-g-\frac{k}{m}x^\frac{3}{2}-\frac{c}{m} \boxed{\dot{y}_{\textsf{p}}}\\
\end{aligned}
}
$$
$\ddot \phi$ depends on whether the friction is static or kinetic.

\subsection{Friction}
\subsubsection{Kinetic friction}
$$F_{\textsf{fric}}=m\ddot{x}_{\textsf{c}}$$
$$F_{\textsf{fric}}=m(\boxed{\ddot{x}_{\textsf{p}}}+\boxed{\ddot \phi} \ell \cos \phi+ \dot \phi^2 \ell \sin\phi)$$
$$\mu_kN=F_{\textsf{fric}}$$
$$\boxed{F_{\textsf{fric}}=
\mu_km(\ddot{y}_{\textsf{p}}+\ddot \phi \ell \sin\phi-\dot \phi^2 \ell \cos\phi+g)}$$
\vspace{\baselineskip}
Finding $\ddot \phi$ using method \textcircled{1}:
$$I\ddot \phi=N\ell\sin\phi-F_{\textsf{friction}}\ell\cos\phi$$
$$I\ddot \phi=N\ell\sin\phi-\mu_kN\ell\cos\phi$$
$$\ddot \phi=\frac{N\ell(\sin\phi-\mu_k\cos\phi)}{I}$$

$$\boxed{\ddot \phi=\frac{m\ell(\ddot{y}_{\textsf{p}}+\ddot \phi \ell \sin\phi-\dot \phi^2 \ell \cos\phi+g)(\sin\phi-\mu_k\cos\phi)}{I}}$$

\vspace{\baselineskip}
Finding $\ddot \phi$ using method \textcircled{2}:
$$
    \begin{cases}
      N-mg=m(\ddot{y}_{\textsf{p}}+\ddot \phi \ell \sin\phi-\dot \phi^2 \ell \cos\phi)\\
      F_{\textsf{fric}}=
\mu_km(\ddot{y}_{\textsf{p}}+\ddot \phi \ell \sin\phi-\dot \phi^2 \ell \cos\phi+g)\\
      I\ddot \phi=N\ell\sin\phi-F_{\textsf{friction}}\ell\cos\phi
    \end{cases}    
$$

Solving the equation simultaneously for $\ddot\phi$ and rearranging the terms,
$$\boxed{m\ell \sin \theta (g+ \ddot y_p)-m\ell \cos\theta \, \ddot x_p=I\ddot \phi}$$
Solving for $\ddot \phi$, the same solution will be obtained.

\subsubsection{Static friction}
$$\ddot x_p=0$$
$$F_{\textsf{friction}}=m(\boxed{\ddot \phi} \ell \cos \phi+ \dot \phi^2 \ell \sin\phi)$$
Non-slip condition:
$$m(\ddot \phi \ell \cos \phi+ \dot \phi^2 \ell \sin\phi)\leq \mu_sN$$
$$m(\ddot \phi \ell \cos \phi+ \dot \phi^2 \ell \sin\phi)\leq \mu_sm(\ddot{y}_{\textsf{p}}+\ddot \phi \ell \sin\phi-\dot \phi^2 \ell \cos\phi+g)$$
$$\boxed{\mu_s\geq\frac{(\ddot \phi \ell \cos \phi+ \dot \phi^2 \ell \sin\phi)}{(\ddot{y}_{\textsf{p}}+\ddot \phi \ell \sin\phi-\dot \phi^2 \ell \cos\phi+g)}}$$

\vspace{\baselineskip}
Finding $\ddot \phi$:
$$\boxed{m\ell \sin \theta (g+ \ddot y_p)-m\ell \cos\theta \, \ddot x_p=I\ddot \phi}$$
$$\ddot x_p=0$$
Moment of inertia about $I_{\textsf{p}}=I_{\textsf{c}}+m\ell^2$
$$m(g+\ddot y_p)\ell \sin \phi=I_p\ddot \phi$$
$$\ddot \phi=\frac{m(g+\ddot y_p)\ell\cos\phi}{I}$$

\section{Time of collision}
Capsule will leave the ground when normal force becomes 0:
$$0=m(\ddot{y}_{\textsf{p}}+\ddot \phi \ell \sin\phi-\dot \phi^2 \ell \cos\phi+g)$$

\section{Some other things}
$\ell$ is a function of $\theta$:
$$\ell (\theta) = R  \sqrt{2(1+\sin\theta)}$$
\vspace{\baselineskip}

$\phi$ is also a function of $\theta$:
$$\phi(\theta)=-\frac{\pi-2\theta}{4}$$
\vspace{\baselineskip}

$\ell$ is therefore a function of $\phi$:
$$\ell(\phi) = R  \sqrt{2(1+\sin\frac{4\phi+\pi}{2})}$$

\end{document}


